Tactics.v
@@ -47,10 +47,19 @@ Ltac invert HH:=
   intros.
 
 
-(** I find this lemma very useful. 
+(** I find these lemmas very useful. 
     Particularly to prove Proper with iff.*)
 Lemma forall_exists_iff: forall A (P Q: A -> Prop),
     (forall x, P x <-> Q x) -> (exists x, P x) <-> (exists x, Q x).
 Proof.
   intros ? ? ? H1; split; intros [v H2]; eexists; eapply H1; eassumption.
 Qed.
+Lemma forall_exists_if: forall A (P Q: A -> Prop),
+    (forall x, P x -> Q x) -> (exists x, P x) -> (exists x, Q x).
+Proof.
+  intros ? ? ? H1; intros [v H2]; eexists; eapply H1; eassumption.
+Qed.
+Lemma forall_and_if:
+  forall (A A' B B': Prop),
+    (A -> A') -> (B -> B') -> (A /\ B) -> (A' /\ B').
+Proof. tauto. Qed.
